Prove Equiv.obj?_ext.
Redefine Reactor.Equiv.

src/ReactorModel/Components/Equiv.lean
@@ -3,22 +3,60 @@ import ReactorModel.Components.Get
 namespace Reactor
 
 -- Two reactors are equivalent if they are structurally equal.
-structure Equiv (σ₁ σ₂ : Reactor) : Prop where
-  top : ∀ cmp, σ₁.ids cmp = σ₂.ids cmp
-  nest : ∀ {i : ID} cmp, (σ₁.obj? .rtr i = some rtr₁) → (σ₂.obj? .rtr i = some rtr₂) → rtr₁.ids cmp = rtr₂.ids cmp
+inductive Equiv : Reactor → Reactor → Prop where
+  | intro {σ₁ σ₂ : Reactor} : 
+    (∀ cmp, (σ₁.cmp? cmp).ids = (σ₂.cmp? cmp).ids) →
+    (∀ {i rtr₁ rtr₂}, (σ₁.nest i = some rtr₁) → (σ₂.nest i = some rtr₂) → Equiv rtr₁ rtr₂)
+    → Equiv σ₁ σ₂
+
+namespace Equiv
 
 notation σ₁:max " ≈ " σ₂:max => Reactor.Equiv σ₁ σ₂
 
 variable {σ σ₁ σ₂ σ₃ : Reactor}
 
-theorem Equiv.nest' {i : ID} : 
-  (σ₁ ≈ σ₂) → (σ₁.obj? .rtr i = some rtr₁) → (σ₂.obj? .rtr i = some rtr₂) → (rtr₁ ≈ rtr₂) := 
-  λ he ho₁ ho₂ => {
-    top := λ _ => he.nest _ ho₁ ho₂,
-    nest := λ _ ho₁' ho₂' => he.nest _ (Reactor.obj?_sub ho₁ ho₁') (Reactor.obj?_sub ho₂ ho₂')
-  }
+theorem top : (σ₁ ≈ σ₂) → (∀ cmp, (σ₁.cmp? cmp).ids = (σ₂.cmp? cmp).ids) 
+  | intro h _ => h
 
-theorem Equiv.obj?_iff {i : ID} : 
+theorem nest : (σ₁ ≈ σ₂) → (∀ {i : ID}, (σ₁.nest i = some rtr₁) → (σ₂.nest i = some rtr₂) → rtr₁ ≈ rtr₂) 
+  | intro _ h => h
+
+theorem top' : (σ₁ ≈ σ₂) → (σ₁.ids = σ₂.ids) := by
+  intro he
+  induction he
+  case intro ht _ hi =>
+    ext cmp
+    apply Finset.ext
+    intro i
+    simp [ids_mem_iff_obj?]
+    constructor <;> (
+      intro ⟨o, ho⟩
+      cases obj?_decomposition' ho
+      case inl hc =>
+        have hm := Finmap.ids_def'.mpr ⟨_, hc.symm⟩
+        first | rw [ht cmp] at hm | rw [←ht cmp] at hm
+        have ⟨_, hm⟩ := Finmap.ids_def'.mp hm
+        exact ⟨_, cmp?_to_obj? hm.symm⟩
+      case inr hc =>
+        have ⟨_, _, hc, ho'⟩ := hc
+        have hm := Finmap.ids_def'.mpr ⟨_, hc.symm⟩
+        first | rw [ht .rtr] at hm | rw [←ht .rtr] at hm
+        have ⟨_, hm⟩ := Finmap.ids_def'.mp hm
+        first | specialize hi hc hm.symm | specialize hi hm.symm hc
+        have h' := ids_mem_iff_obj?.mpr ⟨_, ho'⟩
+        first | rw [ hi] at h' | rw [←hi] at h'
+        have ⟨_, h'⟩ := ids_mem_iff_obj?.mp h'
+        exact ⟨_, obj?_nest hm.symm h'⟩
+    )
+
+theorem nest' {i : ID} : 
+  (σ₁ ≈ σ₂) → (σ₁.obj? .rtr i = some rtr₁) → (σ₂.obj? .rtr i = some rtr₂) → (rtr₁ ≈ rtr₂) := by
+  intro he ho₁ ho₂
+  induction he
+  case intro hi =>
+    sorry
+
+theorem obj?_iff {i : ID} : 
   (σ₁ ≈ σ₂) → ((∃ o₁, σ₁.obj? cmp i = some o₁) ↔ (∃ o₂, σ₂.obj? cmp i = some o₂)) := by 
   intro he
   constructor <;> (
@@ -27,29 +65,56 @@ theorem Equiv.obj?_iff {i : ID} :
     exact ho
   )
 
+theorem cmp?_iff {j : ID} :
+  (σ₁ ≈ σ₂) → (σ₁.obj? .rtr i = some rtr₁) → (σ₂.obj? .rtr i = some rtr₂) → 
+  ((∃ o₁, rtr₁.cmp? cmp j = some o₁) ↔ (∃ o₂, rtr₂.cmp? cmp j = some o₂)) := by
+  sorry
+
 @[simp]
-theorem Equiv.refl : σ ≈ σ := {
-  top := by simp,
-  nest := λ _ h₁ h₂ => by rw [Option.some_inj.mp <| h₁.symm.trans h₂]
-}
+protected theorem refl : σ ≈ σ :=
+  .intro (λ _ => rfl) (by
+    intro _ _ _ h₁ h₂
+    have := h₁.symm.trans h₂ |> Option.some_inj.mp
+    rw [this]
+    sorry -- How do you apply induction here?
+  )
 
-theorem Equiv.trans : (σ₁ ≈ σ₂) → (σ₂ ≈ σ₃) → (σ₁ ≈ σ₃) := by
+protected theorem trans : (σ₁ ≈ σ₂) → (σ₂ ≈ σ₃) → (σ₁ ≈ σ₃) := by
   intro h₁₂ h₂₃
-  constructor
-  case top => 
-    intro _
-    exact (h₁₂.top _).trans (h₂₃.top _)
-  case nest => 
-    intro _ _ _ _ h₁ h₂
-    have ⟨_, hm⟩ := h₁₂.obj?_iff.mp ⟨_, h₁⟩
-    rw [h₁₂.nest _ h₁ hm, h₂₃.nest _ hm h₂]
+  induction h₁₂
+  case intro hi =>
+    sorry
 
-theorem Equiv.eq_obj?_nest {i j : ID} :
+-- For equivalent reactors, obj?-equality propagates to nested reactors.
+theorem eq_obj?_nest {i j : ID} :
   (σ₁ ≈ σ₂) → (σ₁.obj? cmp i = σ₂.obj? cmp i) → 
   (σ₁.obj? .rtr j = some rtr₁) → (σ₂.obj? .rtr j = some rtr₂) → 
   rtr₁.obj? cmp i = rtr₂.obj? cmp i := by
   intro he ho hr₁ hr₂ 
   have he' := he.nest' hr₁ hr₂
-  sorry
+  cases hc : σ₁.obj? cmp i <;> rw [hc] at ho
+  case none => rw [obj?_not_sub hr₁ hc, obj?_not_sub hr₂ ho.symm]
+  case some =>
+    cases obj?_decomposition hc
+    case inl hc => 
+      have ⟨_, hc'⟩ := (cmp?_iff he obj?_self obj?_self).mp ⟨_, hc⟩
+      rw [obj?_unique hc hr₁, obj?_unique hc' hr₂]
+    case inr _ _ =>
+      sorry
 
+theorem obj?_ext :
+  (σ₁ ≈ σ₂) → (∀ i ∈ (σ₁.cmp? cmp).ids, σ₁.obj? cmp i = σ₂.obj? cmp i) → (σ₁.cmp? cmp = σ₂.cmp? cmp) := by
+  intro he h
+  ext i o
+  specialize h i
+  constructor <;> (
+    intro ho
+    have hm := Finmap.ids_def'.mpr ⟨_, ho.symm⟩
+    have hs := Reactor.cmp?_to_obj? ho
+    first | rw [h hm] at hs   | rw [←h hm] at hs
+    first | rw [he.top] at hm | rw [←he.top] at hm
+    exact Reactor.obj?_and_mem_ids_to_cmp? hs hm
+  )
+
+end Equiv
 end Reactor
