src/lakefile.lean
@@ -6,6 +6,6 @@ package reactor_model where
   dependencies := #[
     {
       name := `mathlib
-      src := Source.git "https://github.com/leanprover-community/mathlib4.git" "7778d96d4291e55e332f2124bda43abc5fae57e3"
+      src := Source.git "https://github.com/leanprover-community/mathlib4.git" "2be753a43b2520ef1967a0c5e5a23192b9dc792f"
     }
   ]
